More.v
@@ -1,3 +1,20 @@
+Parameter ml_neq : val.
+Parameter ml_opp : val.
+Parameter ml_mul : val.
+Parameter ml_div : val.
+Parameter ml_append : val.
+Parameter ml_raise : val.
+  (* .. yet to specify *)
+
+Parameter compare : val. (* todo: until functors are supported *)
+
+
+(*--demo  --todo:update?
+Definition mytag (P:Prop) := P.
+Lemma test_add_tag : True.
+Proof. ltac_add_tag mytag. split. Qed.
+--*)
+
 
 
 (********************************************************************)
@@ -65,3 +82,319 @@ Qed.
   
 
  *)
+
+
+
+(* todo bin: old versions *)
+
+Ltac old_get_spec_intro_x x :=
+  match x with
+     | 1%nat => constr:(spec_intro_1)
+     | 2%nat => constr:(spec_intro_2)
+     | 3%nat => constr:(spec_intro_3)
+     | 4%nat => constr:(spec_intro_4)
+  end.
+
+Ltac old_xintros_core cont1 cont2 cont3 :=
+   let arity := spec_goal_arity tt in
+   let lemma := old_get_spec_intro_x arity in
+   apply lemma; [ instantiate; cont1 tt 
+                | instantiate; cont2 tt 
+                | instantiate; cont3 tt ]. 
+
+Tactic Notation "old_xintros" :=
+  old_xintros_core ltac:(fun _ => try xisspec) 
+               ltac:(fun _ => try xcurried) 
+               ltac:(fun _ => idtac).
+
+Tactic Notation "old_xintros_noauto" :=
+  old_xintros_core ltac:(fun _ => idtac) 
+               ltac:(fun _ => idtac) 
+               ltac:(fun _ => idtac).
+
+
+(*bin
+Notation "'Xhint_do' a" := (tag _ (Some a) _ _)
+  (at level 69, only parsing).
+*)
+  (*
+  | Xcase : Xhint_cmd
+  | Xcases : Xhint_cmd
+  | Xcasenosubst : Xhint_cmd.
+  *)
+
+(*--------------------------------------------------------*)
+(* ** [xfunc]  -- todo: deprecated
+
+Ltac xfunc_core f :=
+  let Pf := fresh "TEMP" in 
+  esplit; split; [ | intros Pf; xret; pattern f; apply Pf ].
+
+Tactic Notation "xfunc" :=
+  intro; let f := get_last_hyp tt in xfunc_core f; try xbody.
+
+Tactic Notation "xfunc" "as" "f" :=
+  intros f; xfunc_core f; try xbody.
+
+*)
+      (*xpat_core_new  todo: deprecated
+      match goal with 
+      | |- ?P /\ ?Q => 
+      | |- forall _, _ => introv H
+      end. *)
+
+(*--todo: deprecated?
+Tactic Notation "xok" := 
+  first [ apply_last_hyp | apply refl_equal ].
+*)
+
+
+(*-------todo: deprecated ----------*)
+
+Tactic Notation "xweaken_post" constr(P') := 
+  match goal with
+  |- tag _ _ _ ?P => asserts_rewrite (P = P'); [ try apply bool_of_eq | ]
+  end.
+
+Lemma xweaken_post_lemma : forall T O A (F:(A->Prop)->Prop) (P Q:A->Prop),
+  tag T O F Q -> P = Q -> tag T O F P.
+Proof. intros. subst~. Qed.
+
+Tactic Notation "xweaken_post" := 
+  eapply xweaken_post_lemma; [ | try apply bool_of_eq ].
+
+
+(* --old
+
+Ltac xgo_core optStopAt :=
+  first [
+  let tag := ltac_get_tag tt in
+  let label := ltac_get_label tt in
+  match optStopAt with
+  | Some label => fail
+  | _ => 
+  match tag with
+  | tag_ret => xret
+  | tag_fail => xfail
+  | tag_done => split
+  | tag_apply => xapp_old
+  | tag_let => xlet
+  | tag_letfun => fail
+  | tag_body => fail
+  | tag_letrec => fail
+  | tag_case => xcases_real
+  | tag_if => xif
+  | tag_alias => xalias
+  | tag_toplet => fail
+  | tag_match ?n => xmatch
+  | tag_topfun  => fail
+  end end
+  | let f := spec_goal_fun tt in xcf f
+  | progress(intros) ].
+
+
+Ltac xgo_repeat optStopAt n :=
+  match nat_from_number n with
+  | 0%nat => idtac
+  | S ?n' => xgo_core optStopAt; instantiate;
+             try xgo_repeat optStopAt n'
+  end.
+
+Tactic Notation "xgo" := 
+  xgo_repeat (@None tag_name) (100%nat).
+
+Tactic Notation "xgo" constr(nOrStopAt) := 
+  match type of nOrStopAt with
+  | tag_name => xgo_repeat nOrStopAt (100%nat)
+  | _ => xgo_repeat (@None tag_name) nOrStopAt
+  end.
+
+Tactic Notation "xgon" constr(n) := 
+  xgo_repeat (@None tag_name) n.
+
+Tactic Notation "xgo" "~" := xgo; xauto~; instantiate; xauto~.
+Tactic Notation "xgo" "*" := xgo; xauto*; instantiate; xauto*.
+Tactic Notation "xgo" "~" constr(stopAt) := xgo stopAt; xauto~; instantiate; xauto~.
+Tactic Notation "xgo" "*" constr(stopAt) := xgo stopAt; xauto*; instantiate; xauto*.
+Tactic Notation "xgon" "~" constr(n) := xgon n; xauto~; instantiate; xauto~.
+Tactic Notation "xgon" "*" constr(n) := xgon n; xauto*; instantiate; xauto*.
+
+Tactic Notation "xgos" := xgo 1; try solve [ xgo~ ]. 
+Tactic Notation "xgos" "~" := xgo 1; try solve [ xgo~ ].
+Tactic Notation "xgos" "*" := xgo 1; try solve [ xgo* ].
+
+*)
+
+Axiom foreach_weaken : forall A (P Q:A->Prop) (E:set A),
+  foreach P E -> P ==> Q -> foreach Q E.
+Axiom foreach_union_inv : forall A (P:A->Prop) (E F:set A),
+  foreach P (E \u F) -> foreach P E /\ foreach P F.
+Axiom foreach_union_eq : forall A (P:A->Prop) (E F:set A),
+  foreach P (E \u F) = (foreach P E /\ foreach P F).
+Axiom foreach_single_eq : forall A (P:A->Prop) (X:A),
+  foreach P (\{X}:set A) = P X.
+(* new versions *)
+
+
+Hint Rewrite foreach_union_eq : rew_foreach.
+Tactic Notation "rew_foreach" hyp(H) := autorewrite with rew_foreach in H.
+Tactic Notation "rew_foreach" := autorewrite with rew_foreach.
+
+Tactic Notation "rew_foreach" "~" constr(H) :=
+  rew_foreach H; auto~.
+Tactic Notation "rew_foreach" "*" constr(H) :=
+  rew_foreach H; auto*.
+
+
+(*--------------------------------------------------------*)
+(* ** [xapply_old] *)
+
+Ltac xapply_old_of_core H cont :=
+   let arity_goal := spec_goal_arity tt in
+   let arity_hyp := spec_term_arity H in
+   let lemma := get_spec_elim_x_y arity_hyp arity_goal in
+   eapply lemma; [ apply H | instantiate; cont tt ].
+
+Ltac xapply_old_core cont := (* todo: cut in pieces *)
+  let f := spec_goal_fun tt in
+  first [ let H := get_spec_hyp f in 
+          first [ xapply_old_of_core H cont | fail 2 ]
+        | let H := get_app_hyp f in 
+          let n := spec_term_arity H in
+          let m := spec_goal_arity tt in
+          let W := get_app_weaken_x n in
+          let L := get_app_intro_x_y n m in
+          first [ apply L; first [ sapply H
+                                 | substs; sapply H
+                (* todo: apply H modulo equality on arguments *)
+                                 | eapply W; [ sapply H | ] ]; 
+                  try cont tt
+                | fail 2 ]
+          (* limitation: continuation applied on premises of H *)
+        | xfind f; let H := fresh in 
+          intro H; xapply_old_of_core H cont; clear H
+        | fail 1 "cannot find a specification" ].
+
+(* old
+Ltac xapply_old_core cont :=
+  let f := spec_goal_fun tt in
+  first [ let H := get_spec_hyp f in 
+          first [ xapply_old_of_core H cont | fail 2 ]
+        | xfind f; let H := fresh in 
+          intro H; xapply_old_of_core H cont; clear H
+        | fail 1 "cannot find a specification" ].
+*)
+
+Ltac xapply_old_pre := 
+  match ltac_get_tag tt with
+  | tag_apply => xuntag tag_apply
+  | tag_let => xlet; xuntag tag_apply
+  end.  
+
+Tactic Notation "xapply_old" "by" tactic(cont) := 
+   xapply_old_pre; xapply_old_core cont.
+Tactic Notation "xapply_old" constr(H) "by" tactic(cont) :=
+   xapply_old_pre; xapply_old_of_core H cont.
+Tactic Notation "xapply_old" := 
+   xapply_old by (fun _ => idtac).
+Tactic Notation "xapply_old" constr(H) :=
+   xapply_old H by (fun _ => idtac).
+
+
+
+(*--------------------------------------------------------*)
+(* ** [xapp_old] *)
+
+Tactic Notation "xapp_old" := 
+  xapply_old by (fun _ => xweak).
+Tactic Notation "xapp_old" "as" :=
+  xapply_old by (fun _ => xweak as).
+Tactic Notation "xapp_old" "as" ident(x) :=
+  xapply_old by (fun _ => xweak as x).
+Tactic Notation "xapp_old" "as" ident(x) ident(Hx) := 
+  xapply_old by (fun _ => xweak as x Hx).
+Tactic Notation "xapp_olds" := 
+  xapply_old by (fun _ => xweaks).
+
+Tactic Notation "xapp_old" constr(S) := 
+  xapply_old S by (fun _ => xweak).
+Tactic Notation "xapp_old" constr(S) "as" :=
+  xapply_old S by (fun _ => xweak as).
+Tactic Notation "xapp_old" constr(S) "as" ident(x) :=
+  xapply_old by (fun _ => xweak as x).
+Tactic Notation "xapp_old" constr(S) "as" ident(x) ident(Hx) := 
+  xapply_old S by (fun _ => xweak as x Hx).
+Tactic Notation "xapp_olds" constr(S) := 
+  xapply_old S by (fun _ => xweaks).
+
+Tactic Notation "xapp_old" "~" := xapp_old; xauto~.
+Tactic Notation "xapp_old" "*" := xapp_old; xauto*.
+Tactic Notation "xapp_olds" "~" := xapp_olds; xauto~.
+Tactic Notation "xapp_olds" "*" := xapp_olds; xauto*.
+Tactic Notation "xapp_old" "~" "as" ident(x) := xapp_old as x; auto~.
+Tactic Notation "xapp_old" "*" "as" ident(x) := xapp_old as x; auto*.
+Tactic Notation "xapp_old" "~" constr(S) := xapp_old S; xauto~.
+Tactic Notation "xapp_old" "*" constr(S) := xapp_old S; xauto*.
+Tactic Notation "xapp_olds" "~" constr(S) := xapp_olds S; xauto~.
+Tactic Notation "xapp_olds" "*" constr(S) := xapp_olds S; xauto*.
+Tactic Notation "xapp_old" "~" constr(S) "as" ident(x) := xapp_old S as x; xauto~.
+Tactic Notation "xapp_old" "*" constr(S) "as" ident(x) := xapp_old S as x; xauto*.
+
+(************************************************************)
+(* ** [xcmp] -- TODO: doc *)
+
+Tactic Notation "xcmp" "as" ident(x) :=
+  let Px := fresh "TEMP" in 
+  let R1 := fresh "R1" x in let R2 := fresh "R2" x in
+  xlet as x Px; [ xapp_old | instantiate; destruct Px as [R1 R2]; xif ]. 
+
+Tactic Notation "xcmp" :=
+  let x := fresh "r" in xcmp as x.
+Ltac get_spec_elim_x_y x y :=
+  match constr:(x,y) with
+     | (1%nat,1%nat) => constr:(spec_elim_1_1)
+     | (1%nat,2%nat) => constr:(spec_elim_1_2)
+     | (1%nat,3%nat) => constr:(spec_elim_1_3)
+     | (1%nat,4%nat) => constr:(spec_elim_1_4)
+     | (2%nat,1%nat) => constr:(spec_elim_2_1)
+     | (2%nat,2%nat) => constr:(spec_elim_2_2)
+     | (2%nat,3%nat) => constr:(spec_elim_2_3)
+     | (2%nat,4%nat) => constr:(spec_elim_2_4)
+     | (3%nat,1%nat) => constr:(spec_elim_3_1)
+     | (3%nat,2%nat) => constr:(spec_elim_3_2)
+     | (3%nat,3%nat) => constr:(spec_elim_3_3)
+     | (3%nat,4%nat) => constr:(spec_elim_3_4)
+     | (4%nat,1%nat) => constr:(spec_elim_4_1)
+     | (4%nat,2%nat) => constr:(spec_elim_4_2)
+     | (4%nat,3%nat) => constr:(spec_elim_4_3)
+     | (4%nat,4%nat) => constr:(spec_elim_4_4)
+   end.
+
+
+(*
+Ltac xapp_cont_r_with E solver := (* todo factorize with above *)
+  let R := fresh "R" in let HR := fresh "HR" in intros R HR;
+  instantiate; cbv beta in HR;    (*needs instantiate?*)
+  match list_boxer_of E with
+  | (>>>) => sapply HR; clear R HR; solver tt
+  | ?E' => applys (boxer HR :: E'); try clear R HR; solver tt
+  | _ => idtac
+  end.
+
+Ltac xapp_cont_r_with E solver := (* todo factorize with above *)
+  let R := fresh "R" in let HR := fresh "HR" in intros R HR;
+  instantiate; cbv beta in HR;    (*needs instantiate?*)
+  match list_boxer_of E with
+  | (>>>) => sapply HR; clear R HR; solver tt
+  | ?E' => applys (boxer HR :: E'); try clear R HR; solver tt
+  | ?E' => let M := fresh "TEMP" in forwards: (boxer HR :: E'); 
+     match goal with
+     | |- R _ => first [ apply M | fail 1 ]
+     | |- _ => try clear R HR; solver tt
+     end
+  | _ => idtac
+  end.
+todo: check next version always ok *)
+
+
+
