FuncTactics.v
@@ -1,16 +1,6 @@
 Set Implicit Arguments.
 Require Export FuncDefs FuncPrint FuncPrim.
 
-Hint Extern 1 (@rep _ _ _ _ _) => simpl.
-
-(* todo: move to libtactics *)
-
-Ltac list_boxer_of E :=
-  match type of E with 
-  | List.list Boxer => constr:(E)
-  | _ => constr:((boxer E)::nil)
-  end.
-
 
 (********************************************************************)
 (* ** Tactics *)
@@ -123,27 +113,7 @@ Ltac get_app_spec_x n :=
 
 (** Returns the lemma [spec_elim_n_m] *)
 
-Ltac get_spec_elim_x_y x y :=
-  match constr:(x,y) with
-     | (1%nat,1%nat) => constr:(spec_elim_1_1)
-     | (1%nat,2%nat) => constr:(spec_elim_1_2)
-     | (1%nat,3%nat) => constr:(spec_elim_1_3)
-     | (1%nat,4%nat) => constr:(spec_elim_1_4)
-     | (2%nat,1%nat) => constr:(spec_elim_2_1)
-     | (2%nat,2%nat) => constr:(spec_elim_2_2)
-     | (2%nat,3%nat) => constr:(spec_elim_2_3)
-     | (2%nat,4%nat) => constr:(spec_elim_2_4)
-     | (3%nat,1%nat) => constr:(spec_elim_3_1)
-     | (3%nat,2%nat) => constr:(spec_elim_3_2)
-     | (3%nat,3%nat) => constr:(spec_elim_3_3)
-     | (3%nat,4%nat) => constr:(spec_elim_3_4)
-     | (4%nat,1%nat) => constr:(spec_elim_4_1)
-     | (4%nat,2%nat) => constr:(spec_elim_4_2)
-     | (4%nat,3%nat) => constr:(spec_elim_4_3)
-     | (4%nat,4%nat) => constr:(spec_elim_4_4)
-   end.
-
-Ltac get_new_spec_elim_x_y x y := (* todo: temp *)
+Ltac get_spec_elim_x_y x y := 
   match constr:(x,y) with 
      | (1%nat,1%nat) => constr:(spec_elim_1_1')
      | (1%nat,2%nat) => constr:(spec_elim_1_2')
@@ -516,12 +486,6 @@ Tactic Notation "xleteq" :=
     ltac:(xlet_intro2_simpl).
 
 
-(*--todo: deprecated?
-Tactic Notation "xok" := 
-  first [ apply_last_hyp | apply refl_equal ].
-*)
-
-
 (*--------------------------------------------------------*)
 (* ** [xret], [xfail], [xdone] *)
 
@@ -628,7 +592,7 @@ Ltac xapp_pre cont :=
 Ltac xapp_spec_core H cont_r cont_w :=
    let arity_goal := spec_goal_arity tt in
    let arity_hyp := spec_term_arity H in
-   let lemma := get_new_spec_elim_x_y arity_hyp arity_goal in
+   let lemma := get_spec_elim_x_y arity_hyp arity_goal in
    first [ eapply lemma; [ apply H 
                          | apply post_le_intro; instantiate; cont_w tt ]
          | eapply lemma; [ apply H 
@@ -673,32 +637,6 @@ Ltac xapp_cont_r E :=
   | _ => idtac
   end.
 
-(*
-Ltac xapp_cont_r_with E solver := (* todo factorize with above *)
-  let R := fresh "R" in let HR := fresh "HR" in intros R HR;
-  instantiate; cbv beta in HR;    (*needs instantiate?*)
-  match list_boxer_of E with
-  | (>>>) => sapply HR; clear R HR; solver tt
-  | ?E' => applys (boxer HR :: E'); try clear R HR; solver tt
-  | _ => idtac
-  end.
-
-Ltac xapp_cont_r_with E solver := (* todo factorize with above *)
-  let R := fresh "R" in let HR := fresh "HR" in intros R HR;
-  instantiate; cbv beta in HR;    (*needs instantiate?*)
-  match list_boxer_of E with
-  | (>>>) => sapply HR; clear R HR; solver tt
-  | ?E' => applys (boxer HR :: E'); try clear R HR; solver tt
-  | ?E' => let M := fresh "TEMP" in forwards: (boxer HR :: E'); 
-     match goal with
-     | |- R _ => first [ apply M | fail 1 ]
-     | |- _ => try clear R HR; solver tt
-     end
-  | _ => idtac
-  end.
-todo: check next version always ok *)
-
-
 Ltac xapp_cont_r_with E solver := (* todo factorize with above *)
   let R := fresh "R" in let HR := fresh "HR" in intros R HR;
   instantiate; cbv beta in HR;    (*needs instantiate?*)
@@ -708,7 +646,6 @@ Ltac xapp_cont_r_with E solver := (* todo factorize with above *)
   | ?E' => fapplys (boxer HR :: E'); try clear R HR; solver tt 
   | _ => idtac
   end.
-
 
 (* todo: use an option to factorize with and without spec *)
 
@@ -782,61 +719,6 @@ Tactic Notation "xapp_spec" "*" constr(H) constr(E) :=
 
 
 (*--------------------------------------------------------*)
-(* ** [xapply_old] *)
-
-Ltac xapply_old_of_core H cont :=
-   let arity_goal := spec_goal_arity tt in
-   let arity_hyp := spec_term_arity H in
-   let lemma := get_spec_elim_x_y arity_hyp arity_goal in
-   eapply lemma; [ apply H | instantiate; cont tt ].
-
-Ltac xapply_old_core cont := (* todo: cut in pieces *)
-  let f := spec_goal_fun tt in
-  first [ let H := get_spec_hyp f in 
-          first [ xapply_old_of_core H cont | fail 2 ]
-        | let H := get_app_hyp f in 
-          let n := spec_term_arity H in
-          let m := spec_goal_arity tt in
-          let W := get_app_weaken_x n in
-          let L := get_app_intro_x_y n m in
-          first [ apply L; first [ sapply H
-                                 | substs; sapply H
-                (* todo: apply H modulo equality on arguments *)
-                                 | eapply W; [ sapply H | ] ]; 
-                  try cont tt
-                | fail 2 ]
-          (* limitation: continuation applied on premises of H *)
-        | xfind f; let H := fresh in 
-          intro H; xapply_old_of_core H cont; clear H
-        | fail 1 "cannot find a specification" ].
-
-(* old
-Ltac xapply_old_core cont :=
-  let f := spec_goal_fun tt in
-  first [ let H := get_spec_hyp f in 
-          first [ xapply_old_of_core H cont | fail 2 ]
-        | xfind f; let H := fresh in 
-          intro H; xapply_old_of_core H cont; clear H
-        | fail 1 "cannot find a specification" ].
-*)
-
-Ltac xapply_old_pre := 
-  match ltac_get_tag tt with
-  | tag_apply => xuntag tag_apply
-  | tag_let => xlet; xuntag tag_apply
-  end.  
-
-Tactic Notation "xapply_old" "by" tactic(cont) := 
-   xapply_old_pre; xapply_old_core cont.
-Tactic Notation "xapply_old" constr(H) "by" tactic(cont) :=
-   xapply_old_pre; xapply_old_of_core H cont.
-Tactic Notation "xapply_old" := 
-   xapply_old by (fun _ => idtac).
-Tactic Notation "xapply_old" constr(H) :=
-   xapply_old H by (fun _ => idtac).
-
-
-(*--------------------------------------------------------*)
 (* ** [xweak] *)
 
 Ltac xweak_partial cont := 
@@ -878,46 +760,6 @@ Tactic Notation "xweaks" :=
      | let x := fresh "x" in let Hx := fresh "P" x in 
        intros x Hx; instantiate; cbv beta in Hx; try if_eq in Hx;
        try substs x ]).
-
-
-(*--------------------------------------------------------*)
-(* ** [xapp_old] *)
-
-Tactic Notation "xapp_old" := 
-  xapply_old by (fun _ => xweak).
-Tactic Notation "xapp_old" "as" :=
-  xapply_old by (fun _ => xweak as).
-Tactic Notation "xapp_old" "as" ident(x) :=
-  xapply_old by (fun _ => xweak as x).
-Tactic Notation "xapp_old" "as" ident(x) ident(Hx) := 
-  xapply_old by (fun _ => xweak as x Hx).
-Tactic Notation "xapp_olds" := 
-  xapply_old by (fun _ => xweaks).
-
-Tactic Notation "xapp_old" constr(S) := 
-  xapply_old S by (fun _ => xweak).
-Tactic Notation "xapp_old" constr(S) "as" :=
-  xapply_old S by (fun _ => xweak as).
-Tactic Notation "xapp_old" constr(S) "as" ident(x) :=
-  xapply_old by (fun _ => xweak as x).
-Tactic Notation "xapp_old" constr(S) "as" ident(x) ident(Hx) := 
-  xapply_old S by (fun _ => xweak as x Hx).
-Tactic Notation "xapp_olds" constr(S) := 
-  xapply_old S by (fun _ => xweaks).
-
-Tactic Notation "xapp_old" "~" := xapp_old; xauto~.
-Tactic Notation "xapp_old" "*" := xapp_old; xauto*.
-Tactic Notation "xapp_olds" "~" := xapp_olds; xauto~.
-Tactic Notation "xapp_olds" "*" := xapp_olds; xauto*.
-Tactic Notation "xapp_old" "~" "as" ident(x) := xapp_old as x; auto~.
-Tactic Notation "xapp_old" "*" "as" ident(x) := xapp_old as x; auto*.
-Tactic Notation "xapp_old" "~" constr(S) := xapp_old S; xauto~.
-Tactic Notation "xapp_old" "*" constr(S) := xapp_old S; xauto*.
-Tactic Notation "xapp_olds" "~" constr(S) := xapp_olds S; xauto~.
-Tactic Notation "xapp_olds" "*" constr(S) := xapp_olds S; xauto*.
-Tactic Notation "xapp_old" "~" constr(S) "as" ident(x) := xapp_old S as x; xauto~.
-Tactic Notation "xapp_old" "*" constr(S) "as" ident(x) := xapp_old S as x; xauto*.
-
 
 (*--------------------------------------------------------*)
 (* ** [xinduction] *)
@@ -1123,21 +965,6 @@ Tactic Notation "xfun_induction_nointro" constr(S) constr(I) :=
 
 
 (*--------------------------------------------------------*)
-(* ** [xfunc]  -- todo: deprecated
-
-Ltac xfunc_core f :=
-  let Pf := fresh "TEMP" in 
-  esplit; split; [ | intros Pf; xret; pattern f; apply Pf ].
-
-Tactic Notation "xfunc" :=
-  intro; let f := get_last_hyp tt in xfunc_core f; try xbody.
-
-Tactic Notation "xfunc" "as" "f" :=
-  intros f; xfunc_core f; try xbody.
-
-*)
-
-(*--------------------------------------------------------*)
 (* ** [xintros] *)
 
 (** [xintros] applies to a goal of the form [Spec_n f K]
@@ -1163,34 +990,6 @@ Tactic Notation "xintros" :=
 
 Tactic Notation "xintros_noauto" :=
   xintros_core ltac:(fun _ => idtac) 
-               ltac:(fun _ => idtac) 
-               ltac:(fun _ => idtac).
-
-
-(* todo bin: old versions *)
-
-Ltac old_get_spec_intro_x x :=
-  match x with
-     | 1%nat => constr:(spec_intro_1)
-     | 2%nat => constr:(spec_intro_2)
-     | 3%nat => constr:(spec_intro_3)
-     | 4%nat => constr:(spec_intro_4)
-  end.
-
-Ltac old_xintros_core cont1 cont2 cont3 :=
-   let arity := spec_goal_arity tt in
-   let lemma := old_get_spec_intro_x arity in
-   apply lemma; [ instantiate; cont1 tt 
-                | instantiate; cont2 tt 
-                | instantiate; cont3 tt ]. 
-
-Tactic Notation "old_xintros" :=
-  old_xintros_core ltac:(fun _ => try xisspec) 
-               ltac:(fun _ => try xcurried) 
-               ltac:(fun _ => idtac).
-
-Tactic Notation "old_xintros_noauto" :=
-  old_xintros_core ltac:(fun _ => idtac) 
                ltac:(fun _ => idtac) 
                ltac:(fun _ => idtac).
 
@@ -1293,7 +1092,7 @@ Ltac xcleanpat_core :=
 Tactic Notation "xcleanpat" :=
   xcleanpat_core.
 
-(**--to clean up *)
+(**--todo clean up *)
 
 Tactic Notation "xif_core" ident(H) tactic(cont) :=
   xuntag tag_if; split; intros H; fold_bool; [ | cont tt ].
@@ -1477,19 +1276,6 @@ Tactic Notation "ximpl_rep" "as" simple_intropattern(PX):=
    intros x H; xrep in H as X RX PX; xrep.
 
 
-
-(************************************************************)
-(* ** [xcmp] -- TODO: doc *)
-
-Tactic Notation "xcmp" "as" ident(x) :=
-  let Px := fresh "TEMP" in 
-  let R1 := fresh "R1" x in let R2 := fresh "R2" x in
-  xlet as x Px; [ xapp_old | instantiate; destruct Px as [R1 R2]; xif ]. 
-
-Tactic Notation "xcmp" :=
-  let x := fresh "r" in xcmp as x.
-
-
 (************************************************************)
 (* ** [xalias] *)
 
@@ -1517,17 +1303,12 @@ Tactic Notation "xalias_subst" :=
   xalias as x Hx; subst x.
 
 (************************************************************)
-(* ** [temporary] *)
+(* **  *)
 
 Ltac xpat_core_new H cont1 cont2 :=
   xuntag tag_case; split; 
     [ introv H; cont1 H 
     | introv H; xtag_negpat H; cont2 H ].
-      (* todo: deprecated
-      match goal with 
-      | |- ?P /\ ?Q => 
-      | |- forall _, _ => introv H
-      end. *)
 
 Ltac xpat_post H :=
   try solve [ discriminate | false; congruence ]; 
@@ -1537,6 +1318,7 @@ Tactic Notation "xpat" :=
   let H := fresh in
   xpat_core_new H ltac:(fun _ => idtac) ltac:(fun _ => idtac);
   xpat_post H.
+
 
 (************************************************************)
 (* ** [xmatch] *)
@@ -1601,11 +1383,6 @@ Tactic Notation "xmatch_simple_subst_alias" :=
 (************************************************************)
 (* ** [xgo] *)
 
-(*bin
-Notation "'Xhint_do' a" := (tag _ (Some a) _ _)
-  (at level 69, only parsing).
-*)
-
 Inductive Xhint_cmd :=
   | Xstop : Xhint_cmd
   | XstopNoclear : Xhint_cmd
@@ -1620,11 +1397,6 @@ Inductive Xhint_cmd :=
   | Xlet : forall A, A -> Xhint_cmd
   | Xlets : forall A, A -> Xhint_cmd
   | Xsimple : Xhint_cmd.
-  (*
-  | Xcase : Xhint_cmd
-  | Xcases : Xhint_cmd
-  | Xcasenosubst : Xhint_cmd.
-  *)
 
 Inductive Xhint (a : tag_name) (h : Xhint_cmd) :=
   | Xhint_intro : Xhint a h.
@@ -1769,109 +1541,3 @@ Tactic Notation "xgo" "~" constr(a1) constr(h1) "," constr(a2) constr(h2) ","
   add_hint a1 h1; add_hint a2 h2; add_hint a3 h3; add_hint a4 h4; xgo~.
 
 
-(* --old
-
-Ltac xgo_core optStopAt :=
-  first [
-  let tag := ltac_get_tag tt in
-  let label := ltac_get_label tt in
-  match optStopAt with
-  | Some label => fail
-  | _ => 
-  match tag with
-  | tag_ret => xret
-  | tag_fail => xfail
-  | tag_done => split
-  | tag_apply => xapp_old
-  | tag_let => xlet
-  | tag_letfun => fail
-  | tag_body => fail
-  | tag_letrec => fail
-  | tag_case => xcases_real
-  | tag_if => xif
-  | tag_alias => xalias
-  | tag_toplet => fail
-  | tag_match ?n => xmatch
-  | tag_topfun  => fail
-  end end
-  | let f := spec_goal_fun tt in xcf f
-  | progress(intros) ].
-
-
-Ltac xgo_repeat optStopAt n :=
-  match nat_from_number n with
-  | 0%nat => idtac
-  | S ?n' => xgo_core optStopAt; instantiate;
-             try xgo_repeat optStopAt n'
-  end.
-
-Tactic Notation "xgo" := 
-  xgo_repeat (@None tag_name) (100%nat).
-
-Tactic Notation "xgo" constr(nOrStopAt) := 
-  match type of nOrStopAt with
-  | tag_name => xgo_repeat nOrStopAt (100%nat)
-  | _ => xgo_repeat (@None tag_name) nOrStopAt
-  end.
-
-Tactic Notation "xgon" constr(n) := 
-  xgo_repeat (@None tag_name) n.
-
-Tactic Notation "xgo" "~" := xgo; xauto~; instantiate; xauto~.
-Tactic Notation "xgo" "*" := xgo; xauto*; instantiate; xauto*.
-Tactic Notation "xgo" "~" constr(stopAt) := xgo stopAt; xauto~; instantiate; xauto~.
-Tactic Notation "xgo" "*" constr(stopAt) := xgo stopAt; xauto*; instantiate; xauto*.
-Tactic Notation "xgon" "~" constr(n) := xgon n; xauto~; instantiate; xauto~.
-Tactic Notation "xgon" "*" constr(n) := xgon n; xauto*; instantiate; xauto*.
-
-Tactic Notation "xgos" := xgo 1; try solve [ xgo~ ]. 
-Tactic Notation "xgos" "~" := xgo 1; try solve [ xgo~ ].
-Tactic Notation "xgos" "*" := xgo 1; try solve [ xgo* ].
-
-*)
-
-
-
-
-(*-------todo: deprecated ----------*)
-
-Tactic Notation "xweaken_post" constr(P') := 
-  match goal with
-  |- tag _ _ _ ?P => asserts_rewrite (P = P'); [ try apply bool_of_eq | ]
-  end.
-
-Lemma xweaken_post_lemma : forall T O A (F:(A->Prop)->Prop) (P Q:A->Prop),
-  tag T O F Q -> P = Q -> tag T O F P.
-Proof. intros. subst~. Qed.
-
-Tactic Notation "xweaken_post" := 
-  eapply xweaken_post_lemma; [ | try apply bool_of_eq ].
-
-
-
-
-
-
-Axiom foreach_weaken : forall A (P Q:A->Prop) (E:set A),
-  foreach P E -> P ==> Q -> foreach Q E.
-Axiom foreach_union_inv : forall A (P:A->Prop) (E F:set A),
-  foreach P (E \u F) -> foreach P E /\ foreach P F.
-Axiom foreach_union_eq : forall A (P:A->Prop) (E F:set A),
-  foreach P (E \u F) = (foreach P E /\ foreach P F).
-Axiom foreach_single_eq : forall A (P:A->Prop) (X:A),
-  foreach P (\{X}:set A) = P X.
-
-Hint Rewrite foreach_union_eq : rew_foreach.
-Tactic Notation "rew_foreach" hyp(H) := autorewrite with rew_foreach in H.
-Tactic Notation "rew_foreach" := autorewrite with rew_foreach.
-
-Tactic Notation "rew_foreach" "~" constr(H) :=
-  rew_foreach H; auto~.
-Tactic Notation "rew_foreach" "*" constr(H) :=
-  rew_foreach H; auto*.
-
-
-(*- todo: conflit entre types et termes -*)
-
-
-(* todo: pkoi le nom est perdu apres xcf ? *)
